src/Completeness.v
@@ -9,16 +9,22 @@ Require Import Relation_Operators.
 Require Import Coq.Setoids.Setoid.
 Require Import Typing.
 Require Import Infer.
+Require Import MoreGeneral.
 Require Import NewTypeVariable.
 
 Require Import LibTactics.
 
-Lemma id_increases_in_w : forall (e : term) (i i' : id) (G : ctx) (t : ty) (s : substitution),
-                            getState (runInfer_id e G i) = Some i' -> i <= i'.
-  Admitted.
-
-Lemma new_tv_W: forall (e : term) (G : ctx) (i i': id) (t : ty) (s : substitution) rs,
-    (new_tv_ctx G i) -> (runInfer_id e G i) = rs -> getState rs = Some i' ->
-    getResult rs = Some (t, s) -> new_tv_ty t i' /\ new_tv_subst s i'.
+Lemma id_increases_in_w : forall (e : term) (i i' : id) (G : ctx) (tau : ty) (s : substitution),
+                            getResult (runInfer_id e G i) = Some (i', tau, s) -> i <= i'.
 Admitted.
 
+Lemma new_tv_W: forall (e : term) (G : ctx) (i i': id) (t : ty) (s : substitution),
+    (new_tv_ctx G i) -> getResult (runInfer_id e G i) = Some (i, t, s) ->
+    new_tv_ty t i' /\ new_tv_subst s i'.
+Admitted.
+
+Lemma completeness : forall (e : term) (G : ctx) (tau' : ty) (phi : substitution) (i : id),
+    has_type (apply_subst_ctx phi G) e tau' -> new_tv_ctx G i ->
+    exists s tau i' s', getResult (runInfer_id e G i) = Some (i', tau, s) /\ tau' = apply_subst s' tau /\
+                   (forall x : id, x < i -> apply_subst phi (var x) = apply_subst (s ++ s') (var x)).
+Admitted.
